Minor cleanup in Model, prove PMP extract sound

case_study/RiscvPmp/IrisModel.v
@@ -75,7 +75,6 @@ Module RiscvPmpIrisBase <: IrisBase RiscvPmpBase RiscvPmpProgram RiscvPmpSemanti
     Definition memGS : gFunctors -> Set := mcMemGS.
     Definition memΣ : gFunctors := #[gen_heapΣ Addr MemVal ; tracePreΣ Trace].
 
-    Definition liveAddrs := bv.seqBv (@bv.of_nat xlenbits minAddr) lenAddr.
     Lemma NoDup_liveAddrs : NoDup liveAddrs.
     Proof. now eapply Prelude.nodup_fixed. Qed.
 
